src/GC.fst
@@ -1,6 +1,15 @@
 (** Garbage collection *)
 module GC
 
+open Util
+open Set
+open Total
+open AncillaHeap
+open BoolExp
+open Circuit
+open ExprTypes
+open Interpreter
+
 (* Garbage-collected reversible circuit compilation -- experimental *)
 type qubit =
   { id   : int;
@@ -8,12 +17,12 @@ type qubit =
     cval : BoolExp }
 
 val null_q : qubit
-val get_subst : Total.t int qubit -> int -> Tot int
+val get_subst : Partial.t int qubit -> int -> Tot int
 val data_q : int -> Tot qubit
 val anc_q  : int -> Tot qubit
 
 let nullq = { id = 0; ival = BFalse; cval = BFalse }
-let get_subst m = fun i -> (m i).id
+let get_subst m = fun i -> (Partial.find_def m i nullq).id
 let data_q i = { id = i; ival = BVar i; cval = BFalse }
 let anc_q i  = { id = i; ival = BFalse; cval = BFalse }
 
@@ -21,7 +30,7 @@ type circGCState =
   { top    : int;
     ah     : AncHeap;
     gates  : list Gate;
-    symtab : Total.t int qubit }
+    symtab : Partial.t int qubit }
 
 val circGC       : circGCState -> int -> Tot circGCState
 val circGCInit   : circGCState
@@ -29,56 +38,90 @@ val circGCAlloc  : circGCState -> BoolExp -> Tot (int * circGCState)
 val circGCAssign : circGCState -> int -> BoolExp -> Tot circGCState
 val circGCEval   : circGCState -> state -> int -> Tot bool
 
-// The garbage collector needs to:
-//  -compile the current value in place (i.e. ival + cval + cval = ival),
-//  -if the qubit is an ancilla, push it back onto the heap, and
-//  -update the current value of all other bits by substituting q.id with ival + cval
+(* The garbage collector needs to:
+     -compile the current value in place (i.e. ival + cval + cval = ival),
+     -if the qubit is an ancilla, push it back onto the heap, and
+     -update the current value of all other bits by substituting q.id with ival + cval *)
 val garbageCollect : circGCState -> qubit -> Tot circGCState
 let garbageCollect cs q = 
   let (ah', res, ancs, circ) = compileBexp cs.ah q.id q.cval in
   let ah'' = if q.ival = BFalse then insert ah' q.id else ah' in
   let f q' = 
     let subq = fun v -> if v = q.id then BXor (q.ival, q.cval) else BVar v in
-      { id = q'.id; ival = q'.ival; cval = simplify (substBexp q'.cval subq) }
+      { id   = q'.id; 
+        ival = q'.ival; 
+	cval = simplify (substBexpf q'.cval subq) }
   in
-  let symtab' = mapVal f cs.symtab in
-    { top = cs.top; ah = ah''; gates = cs.gates @ circ; symtab = symtab' }
+  let symtab' = Partial.mapVals f cs.symtab in
+    { top    = cs.top; 
+      ah     = ah''; 
+      gates  = cs.gates @ circ; 
+      symtab = symtab' }
 
-let circGCInit = { top = 0; ah = emptyHeap; gates = []; subs = constMap nullq;
-symtab = constMap nullq }
+let circGCInit = 
+  { top    = 0; 
+    ah     = emptyHeap; 
+    gates  = []; 
+    symtab = [] }
+
 let circGCAlloc cs bexp = 
-  let bexp' = simplify (substVar bexp (get_subst cs.symtab)) in
+  let bexp' = simplify (substVarf bexp (get_subst cs.symtab)) in
   let (ah', bit) = popMin cs.ah in
   let (ah'', res, ancs, circ') = compileBexp ah' bit bexp' in
-  let q = { id = bit; ival = BFalse; cval = bexp' } in
+  let q = { id = bit; 
+	    ival = BFalse; 
+	    cval = bexp' } 
+  in
   let top' = cs.top + 1 in
   let gates' = cs.gates @ circ' in
-  let symtab' = update cs.symtab cs.top q in
+  let symtab' = Partial.update cs.symtab cs.top q in
   (cs.top, {top = top'; ah = ah''; gates = gates'; symtab = symtab'})
+
 let circGCAssign cs l bexp =
-  let q = lookup cs.symtab l in
-  let bexp' = simplify (substVar bexp (get_subst cs.symtab)) in
+  let q = Partial.find_def cs.symtab l nullq in
+  let bexp' = simplify (substVarf bexp (get_subst cs.symtab)) in
   let bexpfac = factorAs bexp' q.id in
   match (q.cval, bexpfac) with
     | (BFalse, _)      -> // substitute q.id with BFalse, compile in place
-      let bexp'' = substBexp bexp' (fun v -> if v = q.id then BFalse else BVar v) in
+      let bexp'' = substBexpf bexp' (fun v -> if v = q.id then BFalse else BVar v) in
       let (ah', res, ancs, circ) = compileBexp cs.ah q.id bexp'' in
       let q' = { id = q.id; ival = q.ival; cval = bexp'' } in
-        {top = cs.top; ah = ah'; gates = cs.gates @ circ; symtab = update cs.symtab l q' }
+      let f b =
+	let subq = fun v -> if v = q.id then bexp'' else BVar v in
+	  { id = b.id; 
+	    ival = b.ival; 
+	    cval = simplify (substBexpf b.cval subq) }
+      in
+      let symtab' = Partial.update (Partial.mapVals f cs.symtab) l q' in
+        { top = cs.top; 
+	  ah = ah'; 
+	  gates = cs.gates @ circ; 
+	  symtab = symtab' }
     | (_, Some bexp'') -> // compile in place, substitute q.id with q.id \oplus bexp''
       let (ah', res, ancs, circ') = compileBexp cs.ah q.id bexp'' in
       let q' = { id = q.id; ival = q.ival; cval = simplify (BXor (q.cval, bexp'')) } in
       let f b = 
         let subq = fun v -> if v = q.id then BXor (BVar q.id, bexp'') else BVar v in
-          { id = b.id; ival = b.ival; cval = simplify (substBexp b.cval subq) }
+	  { id = b.id; 
+	    ival = b.ival; 
+	    cval = simplify (substBexpf b.cval subq) }
       in
-      let symtab' = update (mapVal f cs.symtab) l q' in
-        {top = cs.top; ah = ah'; gates = cs.gates @ circ'; symtab = update cs.symtab l q' }
+      let symtab' = Partial.update (Partial.mapVals f cs.symtab) l q' in
+        { top = cs.top; 
+	  ah = ah'; 
+	  gates = cs.gates @ circ'; 
+	  symtab = symtab' }
     | _                -> // Compile out of place, clean q.id
       let (ah', res, ancs, circ') = compileBexp_oop cs.ah bexp' in
       let q' = { id = res; ival = BFalse; cval = bexp' } in
-      let cs' = { top = cs.top; ah = ah'; gates = cs.gates @ circ'; symtab = update cs.symtab l q' } in
+      let cs' = 
+	{ top = cs.top; 
+	  ah = ah'; 
+	  gates = cs.gates @ circ'; 
+	  symtab = Partial.update cs.symtab l q' } 
+      in
         garbageCollect cs' q
+
 let circGCEval cs st i = false
 
 let circGCInterp = {
@@ -96,7 +139,7 @@ let rec allocNcircGC (locs, cs) i =
     let cs' = { top = cs.top + 1;
                 ah = ah';
                 gates = cs.gates;
-                symtab = update cs.symtab cs.top (data_q res) }
+                symtab = Partial.update cs.symtab cs.top (data_q res) }
     in
       allocNcircGC (((LOC cs.top)::locs), cs') (i-1)
 
@@ -107,7 +150,7 @@ let allocTycircGC ty cs = match ty with
     let cs' = { top = cs.top + 1;
                 ah = ah';
                 gates = cs.gates;
-                symtab = update cs.symtab cs.top (data_q res) }
+                symtab = Partial.update cs.symtab cs.top (data_q res) }
     in
       Val (LOC cs.top, cs')
   | GArray n ->
@@ -115,13 +158,26 @@ let allocTycircGC ty cs = match ty with
       Val (ARRAY locs, st')
   | _ -> Err "Invalid parameter type for circuit generation"
 
-val lookup_Lst_gc : Total.t int qubit -> lst:(list GExpr){isVal_lst lst} -> Tot (list int)
+val lookup_Lst_gc : Partial.t int qubit -> lst:(list GExpr){isVal_lst lst} -> Tot (list int)
 let rec lookup_Lst_gc symtab lst = match lst with
   | [] -> []
-  | (LOC l)::xs -> ((lookup symtab l).id)::(lookup_Lst_gc symtab xs)
+  | (LOC l)::xs -> ((Partial.find_def symtab l nullq).id)::(lookup_Lst_gc symtab xs)
+
+(* Scrubs the state with respect to the remainder of the program *)
+let findGarbage gexp cs = Set.diff (Partial.keys cs.symtab) (locs gexp)
+let garbageCollector gexp cs = 
+  let garbage = findGarbage gexp cs in
+  let f cs l = 
+    let q = Partial.find_def cs.symtab l nullq in
+    let cs' = garbageCollect cs q in
+    { top = cs'.top; ah = cs'.ah; gates = cs'.gates; symtab = Partial.remove cs'.symtab l }
+  in
+    cs
+  //Set.fold f cs garbage
 
 val compileGCCirc : config circGCState -> Dv (result (list int * list Gate))
 let rec compileGCCirc (gexp, cs) =
+  let cs = garbageCollector gexp cs in
   if isVal gexp then match gexp with
     | UNIT -> Val ([], [])
     | LAMBDA (x, ty, t) ->
@@ -130,7 +186,7 @@ let rec compileGCCirc (gexp, cs) =
         | Val (v, cs') -> compileGCCirc (substGExpr t x v, cs')
       end
     | LOC l ->
-      let res = lookup cs.symtab l in
+      let res = Partial.find_def cs.symtab l nullq in
         Val ([res.id], cs.gates)
     | ARRAY lst ->
       let res = lookup_Lst_gc cs.symtab lst in
