src/Partial.fst
@@ -4,26 +4,26 @@ open Set
 
 type t (key:Type) (value:Type) = list (key * value)
 
-val dom      : #key:Type -> #value:Type -> t key value -> Tot (set key)
-val cod      : #key:Type -> #value:Type -> t key value -> Tot (set value)
+val keys     : #key:Type -> #value:Type -> t key value -> Tot (set key)
+val vals     : #key:Type -> #value:Type -> t key value -> Tot (set value)
 val defined  : #key:Type -> #value:Type -> t key value -> key -> Tot bool
-//val empty    : #key:Type -> #value:Type -> Tot (t key value)
 val find     : #key:Type -> #value:Type -> t key value -> key -> Tot (option value)
 val find_def : #key:Type -> #value:Type -> t key value -> key -> value -> Tot value
 val update   : #key:Type -> #value:Type -> t key value -> key -> value -> Tot (t key value)
+val remove   : #key:Type -> #value:Type -> t key value -> key -> Tot (t key value)
 val totalize : #key:Type -> #value:Type -> t key value -> value -> Tot (Total.t key value)
+val mapVals  : #key:Type -> #value:Type -> #value':Type -> 
+	       (value -> Tot value) -> t key value -> Tot (t key value')
 
-let rec dom m = match m with
+let rec keys m = match m with
   | []    -> fun _ -> false
-  | x::xs -> fun y -> (fst x) = y || dom xs y
+  | x::xs -> fun y -> (fst x) = y || keys xs y
 
-let rec cod m = match m with
+let rec vals m = match m with
   | []    -> fun _ -> false
-  | x::xs -> fun y -> (snd x) = y || cod xs y
+  | x::xs -> fun y -> (snd x) = y || vals xs y
 
-let defined m k = mem k (dom m)
-
-//let empty = []
+let defined m k = mem k (keys m)
 
 let rec find m k = List.assocT k m
 
@@ -35,9 +35,15 @@ let rec update m k v = match m with
     | [] -> [(k, v)]
     | (k', v')::xs -> if k = k' then (k, v)::xs else (k', v')::(update xs k v)
 
+let rec remove m k = match m with
+  | [] -> []
+  | (k', v')::xs -> if k = k' then xs else (k', v')::(remove xs k)
+
 let totalize m dval =
   { Total.elts = m;
     Total.dval = dval }
+
+let mapVals f m = List.mapT (fun (k, v) -> (k, f v)) m
 
 (** Verification utilities *)
 val lookup   : #key:Type -> #value:Type -> m:t key value -> k:key{defined m k} -> Tot value
